WIP: ex3

theories/opt/ex3.v
@@ -1,12 +1,13 @@
-From stbor.sim Require Import local invariant refl_step.
+From stbor.sim Require Import local invariant refl.
+From stbor.sim Require Import tactics simple program.
+From stbor.sim Require Import refl_step right_step left_step derived_step.
 
 Set Default Proof Using "Type".
 
 (** Moving a write to a mutable reference up across unknown code. *)
 
-(* TODO: check if Free is in the right place *)
 (* Assuming x : &mut i32 *)
-Definition ex3 : function :=
+Definition ex3_unopt : function :=
   fun: ["i"],
     let: "x" := new_place (&mut int) "i" in
     retag_place "x" (RefPtr Mutable) int FnEntry ;;
@@ -39,6 +40,80 @@ Definition ex3_opt_2 : function :=
   .
 
 (* TODO: show refinement to be transitive *)
-Lemma ex3_sim_fun : ⊨ᶠ ex3 ≥ ex3_opt_1.
+Lemma ex3_sim_fun : ⊨ᶠ ex3_unopt ≥ ex3_opt_1.
 Proof.
+  (* We can't use sim_simple because we need to track our stack frame id *)
+  intros fs ft LOOK rarg es et vls vlt σs σt FREL SUBSTs SUBSTt.
+  (* Substitution *)
+  move:(subst_l_is_Some_length _ _ _ _ SUBSTs) (subst_l_is_Some_length _ _ _ _ SUBSTt).
+  rewrite /= => Hls Hlt.
+  destruct vls as [|vs []]; [done| |done].
+  destruct vlt as [|arg []]; [done| |done]. clear Hls Hlt.
+  inversion FREL as [|???? VREL _].
+  clear FREL. specialize (vrel_eq _ _ _ VREL)=>?.
+  simplify_eq. simpl in SUBSTs, SUBSTt. simplify_eq/=.
+  (* Init call *)
+  exists 10%nat. apply sim_body_init_call=>/= Eqcs.
+  (* Alloc local *)
+  sim_apply sim_body_alloc_local => /=.
+  sim_apply sim_body_let=>/=.
+  (* Write local *)
+  sim_apply sim_body_write_local_1; [solve_sim..|].
+  intros sarg ? σs1 σt1. subst arg.
+  sim_apply sim_body_let=>/=.
+  apply: sim_body_result => _.
+  (* Retag a local place *)
+  sim_apply sim_body_let=>/=.
+  apply Forall2_cons_inv in VREL as [AREL _].
+  sim_apply sim_body_let=>/=.
+    (* Copy local place *)
+    sim_apply sim_body_copy_local; [solve_sim..|].
+    sim_apply sim_body_result => /= VALID.
+    (* Retag *)
+    sim_apply sim_body_retag_ref_fn_entry; [simpl; lia|eauto| |done|..].
+    { rewrite -cmra_assoc (cmra_comm (res_cs _ _)) cmra_assoc. eauto. }
+    { eapply arel_mono; [done|..|exact AREL]. solve_res. } clear VALID.
+    move=> l' told tnew hplt α' nxtp' r0 ? _ IS_i InD σs2 σt2 s_new tk _ /=.
+    subst sarg.
+    have IS_O := (IS_i O ltac:(simpl; lia)). rewrite shift_loc_0_nat in IS_O.
+    destruct IS_O as [(ss & st & Eql' & Eqss & Eqst & ARELs) TOP].
+    rewrite insert_empty.
+    (* Write local *)
+    sim_apply sim_body_write_local_1; [solve_sim..|].
+    intros s ?. simplify_eq. simpl.
+  sim_apply sim_body_let=>/=.
+  (* Copy local place *)
+  sim_apply sim_body_copy_local; [solve_sim..|].
+  sim_apply sim_body_result => /= VALID.
+  sim_apply (sim_body_deref _ _ _ _ (ValR _)).
+  move => ?? Eq. symmetry in Eq. simplify_eq/=.
+  (* Write unique of 42 *)
+  sim_apply sim_body_write_unique_1;
+    [done|solve_sim|by eexists|..]; [solve_sim..|].
+  move => σs3 σt3 TOP3 /=.
+  sim_apply sim_body_let=>/=.
+  (* Copy local (right) *)
+  sim_apply_r sim_body_copy_local_r; [solve_sim..|].
+  apply: sim_body_result=>_/=.
+  (* Write protected right *)
+  sim_apply_r sim_body_deref_r =>/=.
+  sim_apply_r sim_body_write_protected_r;
+    [solve_sim..|by rewrite lookup_insert |by rewrite lookup_insert
+    |by eapply (elem_of_dom_2 _ _ _ Eql')|].
+  intros Eqss3 σt3' rt'. simpl.
+  apply: sim_body_result=>_/=.
+  sim_apply sim_body_let_r =>/=.
+  (* Call *)
+  rewrite -(right_id ε op (_ ⋅ rt')).
+  sim_bind (Call _ _) (Call _ _). (* TODO: sim_apply fails to instantiate evars *)
+  apply (sim_body_step_over_call _ _ _ ε _ (ValR _) [] []); [solve_sim..|].
+  move => rf' ? _ _ frs' frt' σs4 σt4 VREL' /= Eqs1 Eqs2 ? _ _. simplify_eq.
+  exists 5%nat.
+  apply: sim_body_result=>_ /=.
+  sim_apply sim_body_let=>/=.
+  (* Copy local (left) *)
+  sim_apply_l sim_body_copy_local_l; [solve_sim..|].
+  apply: sim_body_result=>_/=.
+  (* Write protected left *)
+  sim_apply_l sim_body_deref_l =>/=.
 Abort.
